<?xml version="1.0"?>
<rdf:RDF xmlns="http://www.localhost:3030/OLDCA#"
     xml:base="http://www.localhost:3030/OLDCA"
     xmlns:rdf="http://www.w3.org/1999/02/22-rdf-syntax-ns#"
     xmlns:owl="http://www.w3.org/2002/07/owl#"
     xmlns:xml="http://www.w3.org/XML/1998/namespace"
     xmlns:xsd="http://www.w3.org/2001/XMLSchema#"
     xmlns:rdfs="http://www.w3.org/2000/01/rdf-schema#">
    <owl:Ontology rdf:about="http://www.localhost:3030/OLDCA">
        <owl:versionIRI rdf:resource="http://www.localhost:3030/OLDCA"/>
    </owl:Ontology>
    


    <!-- 
    ///////////////////////////////////////////////////////////////////////////////////////
    //
    // Object Properties
    //
    ///////////////////////////////////////////////////////////////////////////////////////
     -->

    


    <!-- http://www.localhost:3030/OLDCA#hasAnswer -->

    <owl:ObjectProperty rdf:about="http://www.localhost:3030/OLDCA#hasAnswer">
        <owl:inverseOf rdf:resource="http://www.localhost:3030/OLDCA#isAnswerOf"/>
        <rdfs:domain rdf:resource="http://www.localhost:3030/OLDCA#Question"/>
        <rdfs:range rdf:resource="http://www.localhost:3030/OLDCA#Answer"/>
        <rdfs:comment xml:lang="en">The hasAnswer property relates the question to the answer of the question.</rdfs:comment>
        <rdfs:label xml:lang="en">has Answer</rdfs:label>
    </owl:ObjectProperty>
    


    <!-- http://www.localhost:3030/OLDCA#hasAuthor -->

    <owl:ObjectProperty rdf:about="http://www.localhost:3030/OLDCA#hasAuthor">
        <owl:inverseOf rdf:resource="http://www.localhost:3030/OLDCA#isAuthorOf"/>
        <rdfs:domain rdf:resource="http://www.localhost:3030/OLDCA#Questionnaire"/>
        <rdfs:range rdf:resource="http://www.localhost:3030/OLDCA#Author"/>
        <rdfs:comment xml:lang="en">The hasAuthor property relates the questionnaire to one or more author of the questionnaire.</rdfs:comment>
        <rdfs:label xml:lang="en">has Author</rdfs:label>
    </owl:ObjectProperty>
    


    <!-- http://www.localhost:3030/OLDCA#hasQuestion -->

    <owl:ObjectProperty rdf:about="http://www.localhost:3030/OLDCA#hasQuestion">
        <owl:inverseOf rdf:resource="http://www.localhost:3030/OLDCA#isQuestionOf"/>
        <rdfs:domain rdf:resource="http://www.localhost:3030/OLDCA#Questionnaire"/>
        <rdfs:range rdf:resource="http://www.localhost:3030/OLDCA#Question"/>
        <rdfs:comment xml:lang="en">The hasQuestion property relates the questionnaire to one or more question which is contained in it.</rdfs:comment>
        <rdfs:label xml:lang="en">has Question</rdfs:label>
    </owl:ObjectProperty>
    


    <!-- http://www.localhost:3030/OLDCA#hasRelatedQuestionnaire -->

    <owl:ObjectProperty rdf:about="http://www.localhost:3030/OLDCA#hasRelatedQuestionnaire">
        <owl:inverseOf rdf:resource="http://www.localhost:3030/OLDCA#isRelatedQuestionnaireOf"/>
        <rdfs:domain rdf:resource="http://www.localhost:3030/OLDCA#Questionnaire"/>
        <rdfs:range rdf:resource="http://www.localhost:3030/OLDCA#Questionnaire"/>
        <rdfs:comment xml:lang="en">The hasRelatedQuestionnaire property relates the questionnaire to one or more related questionnaire that share similar topic.</rdfs:comment>
        <rdfs:label xml:lang="en">has related Questionnaire</rdfs:label>
    </owl:ObjectProperty>
    


    <!-- http://www.localhost:3030/OLDCA#hasSubQuestion -->

    <owl:ObjectProperty rdf:about="http://www.localhost:3030/OLDCA#hasSubQuestion">
        <owl:inverseOf rdf:resource="http://www.localhost:3030/OLDCA#isSubQuestionOf"/>
        <rdfs:domain rdf:resource="http://www.localhost:3030/OLDCA#Question"/>
        <rdfs:range rdf:resource="http://www.localhost:3030/OLDCA#Question"/>
        <rdfs:comment xml:lang="en">The hasSubQuestion property relates the question to one or more subquestions under it.</rdfs:comment>
        <rdfs:label xml:lang="en">has subQuestion</rdfs:label>
    </owl:ObjectProperty>
    


    <!-- http://www.localhost:3030/OLDCA#hasTopic -->

    <owl:ObjectProperty rdf:about="http://www.localhost:3030/OLDCA#hasTopic">
        <owl:inverseOf rdf:resource="http://www.localhost:3030/OLDCA#isTopicOf"/>
        <rdfs:domain rdf:resource="http://www.localhost:3030/OLDCA#Question"/>
        <rdfs:domain rdf:resource="http://www.localhost:3030/OLDCA#Questionnaire"/>
        <rdfs:range rdf:resource="http://www.localhost:3030/OLDCA#Topic"/>
        <rdfs:comment xml:lang="en">The hasTopic property relates the questionnaire or the question to the topic of the questionnaire.</rdfs:comment>
        <rdfs:label xml:lang="en">has Topic</rdfs:label>
    </owl:ObjectProperty>
    


    <!-- http://www.localhost:3030/OLDCA#isAnswerOf -->

    <owl:ObjectProperty rdf:about="http://www.localhost:3030/OLDCA#isAnswerOf">
        <rdfs:domain rdf:resource="http://www.localhost:3030/OLDCA#Answer"/>
        <rdfs:range rdf:resource="http://www.localhost:3030/OLDCA#Question"/>
        <rdfs:comment xml:lang="en">The isAnswerOf property relates the Answer to the question.</rdfs:comment>
        <rdfs:label xml:lang="en">is Answer of</rdfs:label>
    </owl:ObjectProperty>
    


    <!-- http://www.localhost:3030/OLDCA#isAuthorOf -->

    <owl:ObjectProperty rdf:about="http://www.localhost:3030/OLDCA#isAuthorOf">
        <rdfs:domain rdf:resource="http://www.localhost:3030/OLDCA#Author"/>
        <rdfs:range rdf:resource="http://www.localhost:3030/OLDCA#Questionnaire"/>
        <rdfs:comment xml:lang="en">The isAuthorOf property relates the Author to the questionnaire.</rdfs:comment>
        <rdfs:label xml:lang="en">is Author of</rdfs:label>
    </owl:ObjectProperty>
    


    <!-- http://www.localhost:3030/OLDCA#isQuestionOf -->

    <owl:ObjectProperty rdf:about="http://www.localhost:3030/OLDCA#isQuestionOf">
        <rdf:type rdf:resource="http://www.w3.org/2002/07/owl#FunctionalProperty"/>
        <rdfs:domain rdf:resource="http://www.localhost:3030/OLDCA#Question"/>
        <rdfs:range rdf:resource="http://www.localhost:3030/OLDCA#Questionnaire"/>
        <rdfs:comment xml:lang="en">The isQuestionOf property relates the question to one questionnaire.</rdfs:comment>
        <rdfs:label xml:lang="en">is Question of</rdfs:label>
    </owl:ObjectProperty>
    


    <!-- http://www.localhost:3030/OLDCA#isRelatedQuestionnaireOf -->

    <owl:ObjectProperty rdf:about="http://www.localhost:3030/OLDCA#isRelatedQuestionnaireOf">
        <rdfs:domain rdf:resource="http://www.localhost:3030/OLDCA#Questionnaire"/>
        <rdfs:range rdf:resource="http://www.localhost:3030/OLDCA#Questionnaire"/>
        <rdfs:comment xml:lang="en">The hasRelatedQuestionnaire property relates the questionnaire to one or more related questionnaire that share similar topic.</rdfs:comment>
        <rdfs:label xml:lang="en">is related Questionnaire of</rdfs:label>
    </owl:ObjectProperty>
    


    <!-- http://www.localhost:3030/OLDCA#isSubQuestionOf -->

    <owl:ObjectProperty rdf:about="http://www.localhost:3030/OLDCA#isSubQuestionOf">
        <rdfs:comment xml:lang="en">The isSubQuestionOf property relates a subquestion to one or more questions.</rdfs:comment>
        <rdfs:label xml:lang="en">is SubQuestion of</rdfs:label>
    </owl:ObjectProperty>
    


    <!-- http://www.localhost:3030/OLDCA#isTopicOf -->

    <owl:ObjectProperty rdf:about="http://www.localhost:3030/OLDCA#isTopicOf">
        <rdfs:domain rdf:resource="http://www.localhost:3030/OLDCA#Topic"/>
        <rdfs:range rdf:resource="http://www.localhost:3030/OLDCA#Question"/>
        <rdfs:range rdf:resource="http://www.localhost:3030/OLDCA#Questionnaire"/>
        <rdfs:comment xml:lang="en">The isTopicOf property relates the topic with either the questionnaire or the question it is discussed in.</rdfs:comment>
        <rdfs:label xml:lang="en">is Topic of</rdfs:label>
    </owl:ObjectProperty>
    


    <!-- 
    ///////////////////////////////////////////////////////////////////////////////////////
    //
    // Data properties
    //
    ///////////////////////////////////////////////////////////////////////////////////////
     -->

    


    <!-- http://www.localhost:3030/OLDCA#hasFirstName -->

    <owl:DatatypeProperty rdf:about="http://www.localhost:3030/OLDCA#hasFirstName">
        <rdfs:domain rdf:resource="http://www.localhost:3030/OLDCA#Author"/>
        <rdfs:range rdf:resource="http://www.w3.org/2000/01/rdf-schema#Literal"/>
        <rdfs:comment xml:lang="en">the first name of a person.</rdfs:comment>
        <rdfs:isDefinedBy rdf:resource="http://xmlns.com/foaf/0.1/"/>
        <rdfs:label xml:lang="en">firstName</rdfs:label>
    </owl:DatatypeProperty>
    


    <!-- http://www.localhost:3030/OLDCA#hasKeywords -->

    <owl:DatatypeProperty rdf:about="http://www.localhost:3030/OLDCA#hasKeywords">
        <rdfs:domain rdf:resource="http://www.localhost:3030/OLDCA#Questionnaire"/>
        <rdfs:range rdf:resource="http://www.w3.org/2000/01/rdf-schema#Literal"/>
        <rdfs:comment xml:lang="en">Keywords that represent the topic of the questionnaire.</rdfs:comment>
        <rdfs:label xml:lang="en">Keywords</rdfs:label>
        <rdfs:label xml:lang="de">Schlagwoerter</rdfs:label>
    </owl:DatatypeProperty>
    


    <!-- http://www.localhost:3030/OLDCA#hasLastName -->

    <owl:DatatypeProperty rdf:about="http://www.localhost:3030/OLDCA#hasLastName">
        <rdfs:domain rdf:resource="http://www.localhost:3030/OLDCA#Author"/>
        <rdfs:range rdf:resource="http://www.w3.org/2000/01/rdf-schema#Literal"/>
        <rdfs:comment xml:lang="en">The last name of a person.</rdfs:comment>
        <rdfs:label xml:lang="en">lastName</rdfs:label>
    </owl:DatatypeProperty>
    


    <!-- http://www.localhost:3030/OLDCA#hasMiddleName -->

    <owl:DatatypeProperty rdf:about="http://www.localhost:3030/OLDCA#hasMiddleName">
        <rdfs:domain rdf:resource="http://www.localhost:3030/OLDCA#Author"/>
        <rdfs:range rdf:resource="http://www.w3.org/2000/01/rdf-schema#Literal"/>
        <rdfs:comment xml:lang="en">The middle name of a person</rdfs:comment>
        <rdfs:label xml:lang="en">middleName</rdfs:label>
    </owl:DatatypeProperty>
    


    <!-- http://www.localhost:3030/OLDCA#hasNote -->

    <owl:DatatypeProperty rdf:about="http://www.localhost:3030/OLDCA#hasNote">
        <rdfs:domain rdf:resource="http://www.localhost:3030/OLDCA#Questionnaire"/>
        <rdfs:range rdf:resource="http://www.w3.org/2000/01/rdf-schema#Literal"/>
        <rdfs:comment xml:lang="en">A short note associated with the questionnaire.</rdfs:comment>
        <rdfs:label xml:lang="de">Anmerkung</rdfs:label>
        <rdfs:label xml:lang="en">Note</rdfs:label>
    </owl:DatatypeProperty>
    


    <!-- http://www.localhost:3030/OLDCA#hasNumber -->

    <owl:DatatypeProperty rdf:about="http://www.localhost:3030/OLDCA#hasNumber">
        <rdfs:domain rdf:resource="http://www.localhost:3030/OLDCA#Question"/>
        <rdfs:domain rdf:resource="http://www.localhost:3030/OLDCA#Questionnaire"/>
        <rdfs:range rdf:resource="http://www.w3.org/2000/01/rdf-schema#Literal"/>
        <rdfs:comment xml:lang="en">The unique number assigned to the question or the questionnaire</rdfs:comment>
        <rdfs:label xml:lang="en">Number</rdfs:label>
        <rdfs:label xml:lang="de">nummer</rdfs:label>
    </owl:DatatypeProperty>
    


    <!-- http://www.localhost:3030/OLDCA#hasOriginalData -->

    <owl:DatatypeProperty rdf:about="http://www.localhost:3030/OLDCA#hasOriginalData">
        <rdfs:domain rdf:resource="http://www.localhost:3030/OLDCA#Question"/>
        <rdfs:range rdf:resource="http://www.w3.org/2000/01/rdf-schema#Literal"/>
        <rdfs:comment xml:lang="en">The original Question printed on the questionnaire and used during data collection.</rdfs:comment>
        <rdfs:label xml:lang="en">Original Data</rdfs:label>
        <rdfs:label xml:lang="de">originaldaten</rdfs:label>
    </owl:DatatypeProperty>
    


    <!-- http://www.localhost:3030/OLDCA#hasOriginalQuestion -->

    <owl:DatatypeProperty rdf:about="http://www.localhost:3030/OLDCA#hasOriginalQuestion">
        <rdfs:domain rdf:resource="http://www.localhost:3030/OLDCA#Question"/>
        <rdfs:range rdf:resource="http://www.w3.org/2000/01/rdf-schema#Literal"/>
        <rdfs:comment xml:lang="en">The original Question asked</rdfs:comment>
        <rdfs:label xml:lang="en">Original Question</rdfs:label>
        <rdfs:label xml:lang="de">originalfrage</rdfs:label>
    </owl:DatatypeProperty>
    


    <!-- http://www.localhost:3030/OLDCA#hasReleaseDate -->

    <owl:DatatypeProperty rdf:about="http://www.localhost:3030/OLDCA#hasReleaseDate">
        <rdfs:domain rdf:resource="http://www.localhost:3030/OLDCA#Questionnaire"/>
        <rdfs:range rdf:resource="http://www.w3.org/2001/XMLSchema#dateTime"/>
        <rdfs:comment xml:lang="en">The release date of the questionnaire. The date the questionnaire is released for collection of data?</rdfs:comment>
        <rdfs:label xml:lang="de">Freigabe</rdfs:label>
        <rdfs:label xml:lang="en">Release Date</rdfs:label>
    </owl:DatatypeProperty>
    


    <!-- http://www.localhost:3030/OLDCA#hasShortQuestion -->

    <owl:DatatypeProperty rdf:about="http://www.localhost:3030/OLDCA#hasShortQuestion">
        <rdfs:domain rdf:resource="http://www.localhost:3030/OLDCA#Question"/>
        <rdfs:range rdf:resource="http://www.w3.org/2000/01/rdf-schema#Literal"/>
        <rdfs:comment xml:lang="en">The short version of the original Question asked.</rdfs:comment>
        <rdfs:label xml:lang="de">Kurzfrage</rdfs:label>
        <rdfs:label xml:lang="en">Short Question</rdfs:label>
    </owl:DatatypeProperty>
    


    <!-- http://www.localhost:3030/OLDCA#hasTitle -->

    <owl:DatatypeProperty rdf:about="http://www.localhost:3030/OLDCA#hasTitle">
        <rdfs:domain rdf:resource="http://www.localhost:3030/OLDCA#Questionnaire"/>
        <rdfs:range rdf:resource="http://www.w3.org/2000/01/rdf-schema#Literal"/>
        <rdfs:comment xml:lang="en">The title of the questionnaire.</rdfs:comment>
        <rdfs:label xml:lang="de">Titel</rdfs:label>
        <rdfs:label xml:lang="en">Title</rdfs:label>
    </owl:DatatypeProperty>
    


    <!-- http://www.localhost:3030/OLDCA#hasYearOfPublication -->

    <owl:DatatypeProperty rdf:about="http://www.localhost:3030/OLDCA#hasYearOfPublication">
        <rdfs:domain rdf:resource="http://www.localhost:3030/OLDCA#Questionnaire"/>
        <rdfs:range rdf:resource="http://www.w3.org/2001/XMLSchema#dateTime"/>
        <rdfs:comment xml:lang="en">The year in which the questionnaire is published.</rdfs:comment>
        <rdfs:label xml:lang="de">Erscheinungsjahr</rdfs:label>
        <rdfs:label xml:lang="en">Year of Publication</rdfs:label>
    </owl:DatatypeProperty>
    


    <!-- http://www.localhost:3030/OLDCA#isChecked -->

    <owl:DatatypeProperty rdf:about="http://www.localhost:3030/OLDCA#isChecked">
        <rdfs:domain rdf:resource="http://www.localhost:3030/OLDCA#Questionnaire"/>
        <rdfs:range rdf:resource="http://www.w3.org/2001/XMLSchema#boolean"/>
        <rdfs:comment xml:lang="en">indicates the questionnaire is checked?</rdfs:comment>
        <rdfs:label xml:lang="de">Checked</rdfs:label>
        <rdfs:label xml:lang="en">Checked</rdfs:label>
    </owl:DatatypeProperty>
    


    <!-- 
    ///////////////////////////////////////////////////////////////////////////////////////
    //
    // Classes
    //
    ///////////////////////////////////////////////////////////////////////////////////////
     -->

    


    <!-- http://www.localhost:3030/OLDCA#AdditionalQuestionnaire -->

    <owl:Class rdf:about="http://www.localhost:3030/OLDCA#AdditionalQuestionnaire">
        <rdfs:subClassOf rdf:resource="http://www.localhost:3030/OLDCA#Questionnaire"/>
        <rdfs:comment xml:lang="en">Additional Questionnaire is a Questionnaire that is used as a supplementary questionnaire to the systematic questionnaire.</rdfs:comment>
        <rdfs:label xml:lang="en">Additional Questionnaire</rdfs:label>
    </owl:Class>
    


    <!-- http://www.localhost:3030/OLDCA#Answer -->

    <owl:Class rdf:about="http://www.localhost:3030/OLDCA#Answer">
        <rdfs:comment xml:lang="en">An Answer represents a written, spoken or illustrated response to a question.</rdfs:comment>
        <rdfs:label xml:lang="en">Answer</rdfs:label>
    </owl:Class>
    


    <!-- http://www.localhost:3030/OLDCA#Author -->

    <owl:Class rdf:about="http://www.localhost:3030/OLDCA#Author">
        <rdfs:comment xml:lang="en">Authors/ collectors are defined in FOAF ontology and we will reuse the definition provided in FOAF Agent/Author classes.</rdfs:comment>
        <rdfs:label xml:lang="en">Author</rdfs:label>
    </owl:Class>
    


    <!-- http://www.localhost:3030/OLDCA#CulturalQuestion -->

    <owl:Class rdf:about="http://www.localhost:3030/OLDCA#CulturalQuestion">
        <rdfs:subClassOf rdf:resource="http://www.localhost:3030/OLDCA#Question"/>
        <rdfs:comment xml:lang="en">Cultural Question is a Question which asks for a belief of societies, procedures on how to make or prepare things, how to play games, contents of cultural songs, poems used for celebrations etc.</rdfs:comment>
        <rdfs:label xml:lang="en">Cultural Question</rdfs:label>
    </owl:Class>
    


    <!-- http://www.localhost:3030/OLDCA#DescriptionQuestion -->

    <owl:Class rdf:about="http://www.localhost:3030/OLDCA#DescriptionQuestion">
        <rdfs:subClassOf rdf:resource="http://www.localhost:3030/OLDCA#Question"/>
        <rdfs:comment xml:lang="en">Description Question is a Question which asks for a written representation of a given entity. An example of description question could be “What would be the function of X?”.</rdfs:comment>
        <rdfs:label xml:lang="en">Description Question</rdfs:label>
    </owl:Class>
    


    <!-- http://www.localhost:3030/OLDCA#DichotomousQuestion -->

    <owl:Class rdf:about="http://www.localhost:3030/OLDCA#DichotomousQuestion">
        <rdfs:subClassOf rdf:resource="http://www.localhost:3030/OLDCA#Question"/>
        <rdfs:comment xml:lang="en">Dichotomous Question is a Question which asks for a selection of answers from a binary option. It includes Yes/No, Agree/disagree, etc. types of answers for stated questions.</rdfs:comment>
        <rdfs:label xml:lang="en">Dichotomous Question</rdfs:label>
    </owl:Class>
    


    <!-- http://www.localhost:3030/OLDCA#IllustrationQuestion -->

    <owl:Class rdf:about="http://www.localhost:3030/OLDCA#IllustrationQuestion">
        <rdfs:subClassOf rdf:resource="http://www.localhost:3030/OLDCA#Question"/>
        <rdfs:comment xml:lang="en">Illustration Question is a Question which asks for a pictorial, diagrammatic, etc.  representation of a given entity. An example of illustration question could be “What Does X look like?”.</rdfs:comment>
        <rdfs:label xml:lang="en">Illustration Question</rdfs:label>
    </owl:Class>
    


    <!-- http://www.localhost:3030/OLDCA#MetaphoricalQuestion -->

    <owl:Class rdf:about="http://www.localhost:3030/OLDCA#MetaphoricalQuestion">
        <rdfs:subClassOf rdf:resource="http://www.localhost:3030/OLDCA#Question"/>
        <rdfs:comment xml:lang="en">Metaphorical Question is a Question which asks for some conveyed meanings of a given word or expression. Metaphorical questions are related to semasiolgical questions, but they ask for additional interpretation of the expression beyond its obvious meaning.</rdfs:comment>
        <rdfs:label xml:lang="en">Metaphorical Question</rdfs:label>
    </owl:Class>
    


    <!-- http://www.localhost:3030/OLDCA#MorphologicalQuestion -->

    <owl:Class rdf:about="http://www.localhost:3030/OLDCA#MorphologicalQuestion">
        <rdfs:subClassOf rdf:resource="http://www.localhost:3030/OLDCA#Question"/>
        <rdfs:comment xml:lang="en">Morphological Question is a Question which asks about the structure and the formation of words and parts of words. Based on the structure, morphological questions can take various forms.</rdfs:comment>
        <rdfs:label xml:lang="en">Morphological Question</rdfs:label>
    </owl:Class>
    


    <!-- http://www.localhost:3030/OLDCA#MultipleChoiceQuestion -->

    <owl:Class rdf:about="http://www.localhost:3030/OLDCA#MultipleChoiceQuestion">
        <rdfs:subClassOf rdf:resource="http://www.localhost:3030/OLDCA#Question"/>
        <rdfs:comment xml:lang="en">Multiple choice Question is a Question which asks for a selection of one item from a list of three or more potential answers.</rdfs:comment>
        <rdfs:label xml:lang="en">Multiple Choice Question</rdfs:label>
    </owl:Class>
    


    <!-- http://www.localhost:3030/OLDCA#OnomasiologicalQuestion -->

    <owl:Class rdf:about="http://www.localhost:3030/OLDCA#OnomasiologicalQuestion">
        <rdfs:subClassOf rdf:resource="http://www.localhost:3030/OLDCA#Question"/>
        <rdfs:comment xml:lang="en">Onomasiological Question is a Question which asks for the name of a given entity. Onomasiological question may take a form of “how do you call x?”.</rdfs:comment>
        <rdfs:label xml:lang="en">Onomasiological Question</rdfs:label>
    </owl:Class>
    


    <!-- http://www.localhost:3030/OLDCA#PhonologicalQuestion -->

    <owl:Class rdf:about="http://www.localhost:3030/OLDCA#PhonologicalQuestion">
        <rdfs:subClassOf rdf:resource="http://www.localhost:3030/OLDCA#Question"/>
        <rdfs:comment xml:lang="en">Phonological Question is a Question which asks for the pronunciation (Sound), or phonetic representation of words.</rdfs:comment>
        <rdfs:label xml:lang="en">Phonological Question</rdfs:label>
    </owl:Class>
    


    <!-- http://www.localhost:3030/OLDCA#Question -->

    <owl:Class rdf:about="http://www.localhost:3030/OLDCA#Question">
        <rdfs:comment xml:lang="en">A Question represents an expression used to request information.</rdfs:comment>
        <rdfs:label xml:lang="de">Frage</rdfs:label>
        <rdfs:label xml:lang="en">Question</rdfs:label>
    </owl:Class>
    


    <!-- http://www.localhost:3030/OLDCA#Questionnaire -->

    <owl:Class rdf:about="http://www.localhost:3030/OLDCA#Questionnaire">
        <rdfs:comment xml:lang="en">A questionnaire represents a set of questions that are related to each other. A questionnaire contains metadata such as questionnaire identifiers, titles, agents and publication related information.  There are six different types of questionnaire which are treated as the subclasses of Questionnaire class.</rdfs:comment>
        <rdfs:label xml:lang="de">Fragebogen</rdfs:label>
        <rdfs:label xml:lang="en">Questionnaire</rdfs:label>
    </owl:Class>
    


    <!-- http://www.localhost:3030/OLDCA#RankingQuestion -->

    <owl:Class rdf:about="http://www.localhost:3030/OLDCA#RankingQuestion">
        <rdfs:subClassOf rdf:resource="http://www.localhost:3030/OLDCA#Question"/>
        <rdfs:comment xml:lang="en">Ranking Question is a Question which asks to compare entities and rank them in a certain order.</rdfs:comment>
        <rdfs:label xml:lang="en">Ranking Question</rdfs:label>
    </owl:Class>
    


    <!-- http://www.localhost:3030/OLDCA#RatingQuestion -->

    <owl:Class rdf:about="http://www.localhost:3030/OLDCA#RatingQuestion">
        <rdfs:subClassOf rdf:resource="http://www.localhost:3030/OLDCA#Question"/>
        <rdfs:comment xml:lang="en">Rating Question is a Question which asks the respondent to assign a rate (degree of excellence) to a given entity based on a predefined range.</rdfs:comment>
        <rdfs:label xml:lang="en">Rating Question</rdfs:label>
    </owl:Class>
    


    <!-- http://www.localhost:3030/OLDCA#SemasiologicalQuestion -->

    <owl:Class rdf:about="http://www.localhost:3030/OLDCA#SemasiologicalQuestion">
        <rdfs:subClassOf rdf:resource="http://www.localhost:3030/OLDCA#Question"/>
        <rdfs:comment xml:lang="en">Semasiological Question is a Question which asks for the meaning of a given entity. Semasiological question may take a form of “what does x means?”.</rdfs:comment>
        <rdfs:label xml:lang="en">Semasiological Question</rdfs:label>
    </owl:Class>
    


    <!-- http://www.localhost:3030/OLDCA#SyntacticQuestion -->

    <owl:Class rdf:about="http://www.localhost:3030/OLDCA#SyntacticQuestion">
        <rdfs:subClassOf rdf:resource="http://www.localhost:3030/OLDCA#Question"/>
        <rdfs:comment xml:lang="en">Syntactic Question is a Question which asks for a construction of phrases or sentences using a given word or a given idiom. They have the form “Provide a phrase/sentence for/using a word/idiom X”.</rdfs:comment>
        <rdfs:label xml:lang="en">Syntactic Question</rdfs:label>
    </owl:Class>
    


    <!-- http://www.localhost:3030/OLDCA#SystematicQuestionnaire -->

    <owl:Class rdf:about="http://www.localhost:3030/OLDCA#SystematicQuestionnaire">
        <rdfs:subClassOf rdf:resource="http://www.localhost:3030/OLDCA#Questionnaire"/>
        <rdfs:comment xml:lang="en">Systematic Questionnaire is a Questionnaire that is used to collect data. This type of questionnaire is used from the beginning of the data collection process.</rdfs:comment>
        <rdfs:label xml:lang="en">Systematic Questionnaire</rdfs:label>
    </owl:Class>
    


    <!-- http://www.localhost:3030/OLDCA#ThesaurusQuestion -->

    <owl:Class rdf:about="http://www.localhost:3030/OLDCA#ThesaurusQuestion">
        <rdfs:subClassOf rdf:resource="http://www.localhost:3030/OLDCA#Question"/>
        <rdfs:comment xml:lang="en">Thesaurus Question is a Question which asks for a list of words or expressions that are used as synonyms (Sometimes, antonyms) or contrasts of a given entity.</rdfs:comment>
        <rdfs:label xml:lang="en">Thesaurus Question</rdfs:label>
    </owl:Class>
    


    <!-- http://www.localhost:3030/OLDCA#Topic -->

    <owl:Class rdf:about="http://www.localhost:3030/OLDCA#Topic">
        <rdfs:comment xml:lang="en">A Topic represents the main subject of a questionnaire or a question.   A questionnaire may focus on a general topic such as “Food” and a question may cover subtopics such as “Traditional Food”.</rdfs:comment>
        <rdfs:label xml:lang="en">Topic</rdfs:label>
    </owl:Class>
</rdf:RDF>



<!-- Generated by the OWL API (version 4.2.8.20170104-2310) https://github.com/owlcs/owlapi -->

